\documentclass[11pt,a4paper]{scrartcl}


\usepackage[utf8]{inputenc}
\usepackage[ngerman]{babel}
\usepackage{amsmath}
\usepackage{amssymb}
\usepackage{graphicx}
\usepackage{hyperref}
\usepackage{gauss}
\usepackage{stmaryrd}

\renewcommand{\thesubsection}{Exercise \arabic{section}.\arabic{subsection}}
\renewcommand{\thesubsubsection}{(\alph{subsubsection})}

\begin{document}
\author{Pavankumar Deshpande, Dmitrii Panichev, Paul KrÃ¶pke, Daniel Biskup}
\title{Foundations of Audio Signal Processing:}
\subtitle{Exercise sheet 4}
\maketitle

\setcounter{section}{4} %sheet 1
\subsection{} %4.1
\begin{align}
||\sum\limits_{j=1}^{n}x_j|| = (\sum\limits_{j=1}^{n}x_j, \sum\limits_{i=1}^{n}x_i) = \sum\limits_{j=1}^{n} (x_j, \sum\limits_{i=1}^{n}x_i) = \sum\limits_{j=1}^{n} x_j \cdot \sum\limits_{i=1}^{n} x_i = \sum\limits_{j=1}^{n} \sum\limits_{i=1}^{n} x_j \cdot x_i = \sum\limits_{j=1}^{n}  \sum\limits_{i=1}^{n} (x_i, x_j)\\
\text{Because of orthogonality of $x$, $(x_i, x_j) = 0$ for $i \neq j$}\\
\text{So (1) = $\sum\limits_{j=1}^{n} (x_j, x_j) = \sum\limits_{j=1}^{n} ||x_j||^{2}$}
\end{align}

\subsection{} %4.2
\subsubsection{} %a
\begin{align}
d(x, y) = |x - y| = \sqrt{(Re(x) - Re(y))^2 + (Im(x) - Im(y))^2}\\
\text{property 1}\\
(Re(x) - Re(y))^2 \geq 0, (Im(x) - Im(y))^2 \geq 0\, \Rightarrow\\
\sqrt{(Re(x) - Re(y))^2 + (Im(x) - Im(y))^2} \geq 0\\
\text{property 2}\\
\Longrightarrow\\
\sqrt{(Re(x) - Re(y))^2 + (Im(x) - Im(y))^2}= 0 \Rightarrow (Re(x) - Re(y))^2 + (Im(x) - Im(y))^2 = 0\\
\Rightarrow Re(x)=Re(y), Im(x)=Im(y) \Rightarrow x=y \\
\Longleftarrow\\
x=y \Rightarrow Re(x) = Re(y), Im(x) = Im(y) \Rightarrow \sqrt{(Re(x) - Re(y))^2 + (Im(x) - Im(y))^2}= 0\\
\text{So, $d(x, y) = 0 \Leftrightarrow x=y$}\\
\text{property 3}\\
d(x, y) = \sqrt{(Re(x) - Re(y))^2 + (Im(x) - Im(y))^2} =\\
\sqrt{((-1) \cdot (Re(x) - Re(y)))^2 + ((-1) \cdot (Im(x) - Im(y)))^2}=\\
\sqrt{(Re(y) - Re(x))^2 + (Im(y) - Im(x))}^2 = d(y, x)\\
\text{property \, 4}\\
\forall x,\,y,\,z\, \in \mathbb{C} \, |x - z| \leq |x - y| + |y - z| \\
\text{because they can be treated as points on the Eucleadean plane with coordinates Re, Im}\\
\text{All 4 properties hold, so it is a metric}
\end{align}

\subsubsection{} %b
\begin{align}
d(x, y) = |x| \cdot |y|\\
\text{Let x=y. Then } d(x ,x) = |x|^2 = Re(x) + Im(x) \text{ not always equals 0.}\\
\text{Property 3 doesn't hold, so it is not a metric}
\end{align}

\subsubsection{} %c
\begin{align}
d(x, y) = \begin{cases}
   1 &\text{if y $\neq$ x}\\
   0 &\text{else}
\end{cases}\\
\text{Property 1}\\
\text{By definition, d(x, y) is always $\geq$ 0}\\
\text{Property 2}\\
\text{By definition, d(x, x) $\Leftrightarrow$ 0}\\
\text{Property 3}\\
d(x, y) = \begin{cases}
   1 &\text{if y $\neq$ x}\\
   0 &\text{else}
\end{cases}\\
d(y, x) = \begin{cases}
   1 &\text{if x $\neq$ y}\\
   0 &\text{else}
\end{cases}\\
d(x, y) = d(y, x)\\
\text{Property 4}\\
\text{d(x, z) $\in$ $\{$0, 1$\}$, d(x, y) + d(y, z) $\in$ $\{$0, 1, 2$\}$}\\
\text{The only case, where $d(x, z) > d(x, y) +d(y, z)$ is $d(x, z) =1$ and $d(x, y) + d(y, z) = 0$}\\
\text{In this case $x=y=z$, which means $d(x, z) = 0$, which contracicts with $d(x, z) = 1$}\\
\text{So, this case never happens.}\\
\text{All 4 properties hold, so it is a metric}
\end{align}
\end{document}