\documentclass[11pt,a4paper]{scrartcl}


\usepackage[utf8]{inputenc}
\usepackage[ngerman]{babel}
\usepackage{amsmath}
\usepackage{amssymb}
\usepackage{graphicx}
\usepackage{hyperref}
\usepackage{gauss}
\usepackage{stmaryrd}
\renewcommand{\thesubsection}{Exercise \arabic{section}.\arabic{subsection}}
\renewcommand{\thesubsubsection}{(\alph{subsubsection})}
\begin{document}
\author{Pavankumar Deshpande, Dmitrii Panichev, Paul Kr√∂pke, Daniel Biskup}
\title{Foundations of Audio Signal Processing:}
\subtitle{Exercise sheet 1}
\maketitle

\setcounter{section}{1} %sheet 1
\subsection{} %1.1
\subsubsection{} %a
\begin{align}
(4-i)\cdot (2+i)=6+4i-2i-i^2=5+2i
\end{align}

 \subsubsection{} %b
\begin{align}
&\qquad(1+2i)^{-1}=a+bi\hspace{5cm}\big|\cdot(1+2i)\\
\Leftrightarrow&\qquad 1=(a+bi)\cdot(1+2i)=a+2ai+bi+2bi^2\\
\Leftrightarrow& \qquad1+0i=a-2b +(2a+b)i
\end{align}
Only fulfilled by
\begin{align}
&\text{(I)}\qquad\qquad\qquad a-2b=1\\
&\text{(II)}\qquad\qquad\qquad 2a+b=0\quad\Leftrightarrow\quad b=-2a\\
&\text{insert in (I)}\qquad a-2(-2a)=5a=1\quad\Leftrightarrow\quad a=\frac{1}{5}\\
&\text{insert in (II)}\qquad b=-2\frac{1}{5}=\frac{-2}{5}
\end{align}
So it can be concluded that
\begin{align}
(1+2i)^{-1}=\frac{1}{5}-\frac{2}{5}i
\end{align}

\subsubsection{}%c
\begin{align}
&2e^{2\pi i}+e^{i\pi 3/2}=2(\cos(2\pi)+i\sin(2\pi))+\cos\left(\frac{3}{2}\pi\right)+i\sin\left(\frac{3}{2}\pi\right)\\
&=2(1+0i)+0-1i=2-1i
\end{align}

\subsubsection{} %d
\begin{align}
4\left(\frac{1-i}{1+i}\right)^2=4\frac{(1-i)^2}{(1-i)^2}=4\frac{1-2i-1}{1+2i-1}=-4\frac{2i}{2i}=-4+0i
\end{align}
\end{document}